Added version of manual self composition for random oracle (quadratical blowup)

examples/relational/ro.fst
@@ -1,7 +1,7 @@
 (*--build-config
     options:--admit_fsi Set;
     variables:LIB=../../lib;
-    other-files:$LIB/ext.fst $LIB/set.fsi $LIB/heap.fst $LIB/st.fst $LIB/st2.fst $LIB/bytes.fst $LIB/list.fst  
+    other-files:$LIB/ext.fst $LIB/set.fsi $LIB/heap.fst $LIB/st.fst $LIB/st2.fst $LIB/bytes.fst $LIB/list.fst
 
   --*)
 
@@ -20,43 +20,43 @@ type key = b:bytes{length(b)=eta}
 type tag = b:bytes{length(b)=eta}
 
 (* TODO? *)
-(* an abstract relational predicate on correctly-generated entries *) 
-assume logic type safe_key (k0:key) (k1:key) 
-let safe_key_unique = assume (forall k0 k1 k1'. 
+(* an abstract relational predicate on correctly-generated entries *)
+assume logic type safe_key (k0:key) (k1:key)
+let safe_key_unique = assume (forall k0 k1 k1'.
                                (safe_key k0 k1 /\ safe_key k0 k1' ==> k1 = k1'))
-let safe_key_unique' = assume (forall k0 k0' k1. 
+let safe_key_unique' = assume (forall k0 k0' k1.
                                (safe_key k0 k1 /\ safe_key k0' k1 ==> k0 = k0'))
-assume logic type safe (k0:key) (k1:key) (t0:tag) (t1:tag) 
+assume logic type safe (k0:key) (k1:key) (t0:tag) (t1:tag)
 
 
-type alloc = 
+type alloc =
   | Hon: alloc
-  | Adv: alloc (* a "ghost" field recording the first allocator for a given key *) 
+  | Adv: alloc (* a "ghost" field recording the first allocator for a given key *)
 
 type log = map key (alloc * tag)
 
 type state =
-  { bad: bool; (* set iff any allocation has failed, e.g. bumped into the other's table *) 
+  { bad: bool; (* set iff any allocation has failed, e.g. bumped into the other's table *)
     l:log }    (* the map ensures at most one entry per key *)
 
 
-type Ok : log -> log -> Type = 
-  | Null: Ok [] [] 
-  | ConsH: k0:key -> k1:key{safe_key k0 k1} -> t0:tag -> t1:tag{safe k0 k1 t0 t1} 
-           -> log0:log{is_None (assoc k0 log0)} 
-           -> log1:log{is_None (assoc k1 log1)} 
-           -> p: Ok log0 log1 
+type Ok : log -> log -> Type =
+  | Null: Ok [] []
+  | ConsH: k0:key -> k1:key{safe_key k0 k1} -> t0:tag -> t1:tag{safe k0 k1 t0 t1}
+           -> log0:log{is_None (assoc k0 log0)}
+           -> log1:log{is_None (assoc k1 log1)}
+           -> p: Ok log0 log1
            -> Ok ((k0,(Hon,t0))::log0) ((k1,(Hon,t1))::log1)
-  | ConsA: k:key -> t:tag 
-           -> log0:log{is_None (assoc k log0)} 
-           -> log1:log{is_None (assoc k log1)} 
-           -> p: Ok log0 log1 
+  | ConsA: k:key -> t:tag
+           -> log0:log{is_None (assoc k log0)}
+           -> log1:log{is_None (assoc k log1)}
+           -> p: Ok log0 log1
            -> Ok ((k ,(Adv,t ))::log0) ((k, (Adv,t ))::log1)
 
-val ok_adv_eq : l0:log -> l1:log -> p:Ok l0 l1 -> k:key 
-                -> Lemma 
+val ok_adv_eq : l0:log -> l1:log -> p:Ok l0 l1 -> k:key
+                -> Lemma
                    (requires True)
-                   (ensures (forall t. assoc k l0 = Some(Adv, t) <==> 
+                   (ensures (forall t. assoc k l0 = Some(Adv, t) <==>
                                        assoc k l1 = Some(Adv, t)))
 let rec ok_adv_eq l0 l1 p k = match p with
         | Null -> ()
@@ -66,26 +66,26 @@ let rec ok_adv_eq l0 l1 p k = match p with
 assume val ok_witness : l0:log -> l1:log {Ok l0 l1} -> Ok l0 l1
 
 (* Is there any way to show this using the previous lemma? *)
-val ok_adv_eq' : k:key 
-                -> Lemma 
+val ok_adv_eq' : k:key
+                -> Lemma
                    (requires True)
-                   (ensures (forall (l0:log) (l1:log).Ok l0 l1 ==> 
-                              (forall t. assoc k l0 = Some(Adv, t) <==> 
+                   (ensures (forall (l0:log) (l1:log).Ok l0 l1 ==>
+                              (forall t. assoc k l0 = Some(Adv, t) <==>
                                          assoc k l1 = Some(Adv, t))))
 let ok_adv_eq' k = admit ()
 
 val ok_hon_safe : k0:key -> k1:key -> l0:log -> l1:log -> p:Ok l0 l1
-                -> Lemma 
+                -> Lemma
                    (requires (safe_key k0 k1))
                    (ensures ( (is_Some(assoc k0 l0) /\ is_Hon(fst (Some.v(assoc k0 l0)))) <==>
                                is_Some(assoc k1 l1) /\ is_Hon(fst (Some.v(assoc k1 l1)))))
 let rec ok_hon_safe k0 k1 l0 l1 p = match p with
         | Null -> ()
         | ConsH k0' k1' t01 t1' tl0 tl1 p' -> ok_hon_safe k0 k1 tl0 tl1 p'
-        | ConsA k' t' tl0 tl1 p' -> ok_hon_safe k0 k1 tl0 tl1 p' 
+        | ConsA k' t' tl0 tl1 p' -> ok_hon_safe k0 k1 tl0 tl1 p'
 
-val ok_hon_safe' : k0:key -> k1:key 
-                -> Lemma 
+val ok_hon_safe' : k0:key -> k1:key
+                -> Lemma
                    (requires (safe_key k0 k1))
                    (ensures (forall (l0:log) (l1:log). Ok l0 l1 ==>
                               (is_Some(assoc k0 l0) /\ is_Hon(fst (Some.v(assoc k0 l0)))) <==>
@@ -93,33 +93,33 @@ val ok_hon_safe' : k0:key -> k1:key
 let ok_hon_safe' k0 k1 = admit ()
 
 val ok_hon_safe2 : k0:key -> k1:key -> l0:log -> l1:log -> p:Ok l0 l1
-                -> Lemma 
+                -> Lemma
                    (requires (safe_key k0 k1))
-                   (ensures (is_Some(assoc k0 l0) /\ is_Hon(fst(Some.v(assoc k0 l0))) ==> 
-                               is_Some(assoc k1 l1) /\ 
+                   (ensures (is_Some(assoc k0 l0) /\ is_Hon(fst(Some.v(assoc k0 l0))) ==>
+                               is_Some(assoc k1 l1) /\
                                safe k0 k1 (snd(Some.v(assoc k0 l0))) (snd(Some.v(assoc k1 l1)))))
 let rec ok_hon_safe2 k0 k1 l0 l1 p = match p with
         | Null -> ()
         | ConsH k0' k1' t01 t1' tl0 tl1 p' -> ok_hon_safe2 k0 k1 tl0 tl1 p'
-        | ConsA k' t' tl0 tl1 p' -> ok_hon_safe2 k0 k1 tl0 tl1 p' 
+        | ConsA k' t' tl0 tl1 p' -> ok_hon_safe2 k0 k1 tl0 tl1 p'
 
-assume val ok_hon_safe'' : k0:key -> k1:key 
-                -> Lemma 
+assume val ok_hon_safe'' : k0:key -> k1:key
+                -> Lemma
                    (requires (safe_key k0 k1))
-                   (ensures (forall (l0:log) (l1:log). Ok l0 l1 ==> 
-                                (is_Some(assoc k0 l0) /\ is_Hon(fst(Some.v(assoc k0 l0))) ==> 
-                                  is_Some(assoc k1 l1) /\ 
+                   (ensures (forall (l0:log) (l1:log). Ok l0 l1 ==>
+                                (is_Some(assoc k0 l0) /\ is_Hon(fst(Some.v(assoc k0 l0))) ==>
+                                  is_Some(assoc k1 l1) /\
                                   safe k0 k1 (snd(Some.v(assoc k0 l0))) (snd(Some.v(assoc k1 l1))))))
 
-type goodstate (s1:state) (s2:state) = 
+type goodstate (s1:state) (s2:state) =
             s1.bad = true \/ s2.bad = true \/ Ok s1.l s2.l
 
-assume val s : ref state 
-assume val sample_hon : k0:key -> k1:key -> 
+assume val s : ref state
+assume val sample_hon : k0:key -> k1:key ->
                  ST2 (tag * tag)
                    (requires (fun _ -> True))
                    (ensures (fun h2' p h2 -> h2' = h2 /\ safe k0 k1 (fst p) (snd p)))
-assume val sample_adv : unit -> 
+assume val sample_adv : unit ->
                  ST2 (tag * tag)
                    (requires (fun _ -> True))
                    (ensures (fun h2' p h2 -> h2' = h2 /\ fst p = snd p))
@@ -128,49 +128,82 @@ val hash_hon:  k0:key -> k1:key ->
                ST2 (option tag * option tag)
                (requires (fun h2 -> goodstate (sel (fst h2) s) (sel (snd h2) s) /\
                           safe_key k0 k1))
-               (ensures (fun _ p h2 -> (sel (fst h2) s).bad \/ 
-                                       (sel (snd h2) s).bad \/ 
-                                       is_Some (fst p) /\ is_Some (snd p) /\ 
+               (ensures (fun _ p h2 -> (sel (fst h2) s).bad \/
+                                       (sel (snd h2) s).bad \/
+                                       is_Some (fst p) /\ is_Some (snd p) /\
                                           safe k0 k1 (Some.v(fst p)) (Some.v(snd p))))
 
-val hash_adv:  k:key -> 
+val hash_hon2: k0:key -> k1:key ->
+               ST2 (option tag * option tag)
+               (requires (fun h2 -> goodstate (sel (fst h2) s) (sel (snd h2) s) /\
+                          safe_key k0 k1))
+               (ensures (fun _ p h2 -> (sel (fst h2) s).bad \/
+                                       (sel (snd h2) s).bad \/
+                                       is_Some (fst p) /\ is_Some (snd p) /\
+                                          safe k0 k1 (Some.v(fst p)) (Some.v(snd p))))
+
+val hash_adv:  k:key ->
                ST2 (option tag * option tag)
                (requires (fun h2 -> goodstate (sel (fst h2) s) (sel (snd h2) s)))
-               (ensures (fun _ p h2 -> (sel (fst h2) s).bad \/ 
-                                       (sel (snd h2) s).bad \/ 
-                                       is_Some (fst p) /\ is_Some (snd p) /\ 
+               (ensures (fun _ p h2 -> (sel (fst h2) s).bad \/
+                                       (sel (snd h2) s).bad \/
+                                       is_Some (fst p) /\ is_Some (snd p) /\
                                           Some.v(fst p) = Some.v(snd p)))
-                                      
+
 (* workaround for some typing problems... *)
 val add_some : tag -> Tot (option tag)
 let add_some t = Some t
 
-let hash_hon' k r = match assoc k (!s).l with 
+let case_Hon  t     = Some t
+let case_Adv  _     = s:={bad = true; l=(!s).l}; None
+let case_None (k,t) = s:={bad = (!s).bad; l = (k,(Hon,t))::(!s).l}; add_some t
+
+assume val sample_single : unit -> Tot tag
+
+let hash_hon2 k0 k1 =
+  ok_hon_safe' k0 k1;
+  ok_hon_safe'' k0 k1;
+  let l0, l1 = compose2 (fun _ -> (!s).l) (fun _ -> (!s).l) () () in
+  match assoc k0 l0, assoc k1 l1 with
+  | Some (Hon,t0), Some (Hon,t1) -> compose2 (fun x -> case_Hon x) (fun x -> case_Hon x) t0 t1
+  | Some (Hon,t0), Some (Adv,t1) -> compose2 (fun x -> case_Hon x) (fun x -> case_Adv x) t0 ()
+  | Some (Hon,t0), None          -> let t1 = sample_single () in
+                                    compose2 (fun x -> case_Hon x) (fun x -> case_None x) t0 (k1,t1)
+  | Some (Adv,t0), Some (Hon,t1) -> compose2 (fun x -> case_Adv x) (fun x -> case_Hon x) () t0
+  | Some (Adv,t0), Some (Adv,t1) -> compose2 (fun x -> case_Adv x) (fun x -> case_Adv x) () ()
+  | Some (Adv,t0), None          -> let t1 = sample_single () in
+                                    compose2 (fun x -> case_Adv x) (fun x -> case_None x) () (k1,t1)
+  | None         , Some (Hon,t1) -> let t0 = sample_single () in
+                                    compose2 (fun x -> case_None x) (fun x -> case_Hon x) (k0,t0) t1
+  | None         , Some (Adv,t1) -> let t0 = sample_single () in
+                                    compose2 (fun x -> case_None x) (fun x -> case_Adv x) (k0,t0) ()
+  | None         , None          -> let t0, t1 = sample_hon k0 k1 in
+                                    compose2 (fun x -> case_None x) (fun x -> case_None x) (k0,t0) (k1,t1)
+
+let hash_hon' k r = match assoc k (!s).l with
   | Some (Hon,t) -> Some t
   | Some (Adv,t) -> s := {bad = true; l = (!s).l}; None
-  | None         -> let t = r in 
-                    s := {bad = (!s).bad; l= (k,(Hon,t))::(!s).l} ; 
-                    add_some t 
-
-assume val cheat : k0:key -> k1:key -> t0:tag -> t1:tag -> Lemma(safe k0 k1 t0 t1)
+  | None         -> let t = r in
+                    s := {bad = (!s).bad; l= (k,(Hon,t))::(!s).l} ;
+                    add_some t
 
 let hash_hon k0 k1  = ok_hon_safe' k0 k1;
                       ok_hon_safe'' k0 k1;
-                      let r0, r1 = sample_hon k0 k1 in 
-                      (compose2 (fun k -> hash_hon' k r0) 
-                                (fun k -> hash_hon' k r1) 
+                      let r0, r1 = sample_hon k0 k1 in
+                      (compose2 (fun k -> hash_hon' k r0)
+                                (fun k -> hash_hon' k r1)
                                 k0 k1)
 
-let hash_adv' k r =  match assoc k (!s).l with 
-  | Some (Adv,t) -> Some t 
+let hash_adv' k r =  match assoc k (!s).l with
+  | Some (Adv,t) -> Some t
   | Some (Hon,t) -> s := {bad = true; l = (!s).l}; None
-  | None         -> let t = r in 
-                    s := {bad = (!s).bad; l= (k,(Adv,t))::(!s).l} ; 
-                    add_some t 
+  | None         -> let t = r in
+                    s := {bad = (!s).bad; l= (k,(Adv,t))::(!s).l} ;
+                    add_some t
 
 
 let hash_adv k  = ok_adv_eq' k;
-                  let r0, r1 = sample_adv () in 
-                  compose2 (fun k -> hash_adv' k r0) 
-                           (fun k -> hash_adv' k r1) 
+                  let r0, r1 = sample_adv () in
+                  compose2 (fun k -> hash_adv' k r0)
+                           (fun k -> hash_adv' k r1)
                            k k
